\begin{align}
	  c \frac{\partial u}{\partial t} & = \frac{\partial u}{\partial x} \left( \, d \frac{\partial u}{\partial x} \, \right) \,,
	& t & \ > \ 0\,, \;&  x & \ \in \ \big[ \, 0, \, 1 \, \big] \,, \\[3pt]
	  d \, \frac{\partial u}{\partial x} & = \mathrm{Bi} \cdot \left( \, u - u_{\,L} \, \right)  \,,
	& t & \ > \ 0\,, \,& x & = 0 \,, \\[3pt]
	 -d \, \frac{\partial u}{\partial x} & = \mathrm{Bi} \cdot \left( \, u - u_{\,R} \, \right)  \,,
	& t & \ > \ 0\,, \,&   x & = 1 \,, \\[3pt]
	 u & = 1 \,,
	& t & = 0\,, \,& x & \ \in \ \big[ \, 0, \, 1 \, \big] \,.
	\end{align}